@prefix rdfs: <http://www.w3.org/2000/01/rdf-schema#> .
@prefix skos: <http://www.w3.org/2004/02/skos/core#> .

<http://example.org/lvl2_009> a skos:Concept ;
    rdfs:comment "The amount of value an item or a service has in relation to its acceptable cash price for a willing seller and buyer." ;
    skos:broader <http://example.org/lvl1_003> ;
    skos:inScheme <http://example.org/NceaOntology> ;
    skos:notation "lvl2_009" ;
    skos:prefLabel "Monetary" .

<http://example.org/lvl2_010> a skos:Concept ;
    rdfs:comment "The value attributable to an item or a service without relation to any acceptable cash price and for which a fixed or determinable amount of currency is absent (e.g. many ecosystem services, interpersonal good-will, health, etc.)." ;
    skos:broader <http://example.org/lvl1_003> ;
    skos:inScheme <http://example.org/NceaOntology> ;
    skos:notation "lvl2_010" ;
    skos:prefLabel "Non-monetary" .

<http://example.org/lvl1_003> a skos:Concept ;
    rdfs:comment "For the purposes of this search tool, natural capital valuation is defined as the method used to determine the value of an ecosystem service. This can be in non-monetary terms (e.g. heritage values or existence values) or in monetary terms (e.g. market price or willingness to pay)." ;
    skos:inScheme <http://example.org/NceaOntology> ;
    skos:notation "lvl1_003" ;
    skos:prefLabel "Natural capital valuation" ;
    skos:topConceptOf <http://example.org/NceaOntology> .

[] a skos:Collection ;
    skos:member <http://example.org/lvl1_003>,
        <http://example.org/lvl2_009>,
        <http://example.org/lvl2_010> .

